compiler/proofs/modLangProofScript.sml
@@ -2211,11 +2211,11 @@ val prog_to_i1_mods = Q.prove (
 `!l mods tops prog l' mods' tops' prog_i1.
   prog_to_i1 l mods tops prog = (l',mods', tops',prog_i1)
   ⇒
-  FLAT (MAP (λtop. case top of Tmod mn v5 v6 => [mn] | Tdec v7 => []) prog)
+  prog_to_mods prog
   =
-  FLAT (MAP (λprompt. case prompt of Prompt_i1 NONE ds => [] | Prompt_i1 (SOME mn) ds => [mn]) prog_i1)`,
+  prog_i1_to_mods prog_i1`,
  induct_on `prog` >>
- rw [prog_to_i1_def, LET_THM] >>
+ rw [prog_to_i1_def, LET_THM, prog_i1_to_mods_def, prog_to_mods_def] >>
  rw [] >>
  `?w x y z. top_to_i1 l mods tops h = (w,x,y,z)` by metis_tac [pair_CASES] >>
  fs [] >>
@@ -2231,9 +2231,10 @@ val prog_to_i1_mods = Q.prove (
  >- (`?a b c. decs_to_i1 l (SOME s) mods tops l'' = (a,b,c)` by metis_tac [pair_CASES] >>
      fs [])
  >- (`?a b c. decs_to_i1 l (SOME s) mods tops l'' = (a,b,c)` by metis_tac [pair_CASES] >>
-     fs [] >>
+     fs [prog_to_mods_def, prog_i1_to_mods_def] >>
      metis_tac [])
- >- metis_tac []
+ >- (fs [prog_to_mods_def, prog_i1_to_mods_def] >>
+     metis_tac [])
  >- (`?a b c. dec_to_i1 l NONE mods tops d = (a,b,c)` by metis_tac [pair_CASES] >>
      fs []));
 
@@ -2241,14 +2242,14 @@ val prog_to_i1_top_types = Q.prove (
 `!l mods tops prog l' mods' tops' prog_i1.
   prog_to_i1 l mods tops prog = (l',mods', tops',prog_i1)
   ⇒
-  FLAT (MAP (λtop. case top of Tmod v4 v5 v6 => [] | Tdec d => decs_to_types [d]) prog)
+  prog_to_top_types prog
   =
-  FLAT (MAP (λprompt. case prompt of Prompt_i1 NONE ds => decs_to_types_i1 ds | Prompt_i1 (SOME v5) ds => []) prog_i1)`,
+  prog_i1_to_top_types prog_i1`,
  induct_on `prog` >>
  rw [prog_to_i1_def, LET_THM] >>
  rw [] >>
  `?w x y z. top_to_i1 l mods tops h = (w,x,y,z)` by metis_tac [pair_CASES] >>
- fs [] >>
+ fs [prog_to_top_types_def, prog_i1_to_top_types_def] >>
  `?w' x' y' z'. prog_to_i1 w x y prog = (w',x',y',z')` by metis_tac [pair_CASES] >>
  fs [] >>
  rw [] >>
